Splinter/AsyncDiskProgram.s.dfy
@@ -8,6 +8,7 @@ include "../lib/Checksums/CRC32C.s.dfy"
 
 // Disk API Interface to the implementer-supplied program that is getting verified.
 abstract module AsyncDiskProgram {
+  import AllocationMod
   import D = AsyncDisk  // Importing for the interface, not the entire disk
   import CrashTolerantMapSpecMod
 
@@ -20,6 +21,7 @@ abstract module AsyncDiskProgram {
   type RespRead = D.RespRead
   type RespWrite = D.RespWrite
 
+  predicate Mkfs(dv: AllocationMod.DiskView)
   predicate Init(s: Variables)
   predicate Next(s: Variables, s': Variables, uiop: UIOp, dop: DiskOp)
 }
